bloodRep.dfy
@@ -20,17 +20,84 @@ module BloodRep {
     if(bType == 3) {return O;}
   }
   
-  method createBr(bt: BloodType, l: string, day1:int,month1:int,yr1:int, day2:int,month2:int,yr2:int, isOkay: bool) returns (br: BloodRecord)
+  // Create a blood record
+  // TODO make a date addition to automatically set expiry date rather than pass through
+  method createBr(bt: BloodType, l: string, dd1:int,mm1:int,yy1:int, dd2:int,mm2:int,yy2:int, isOkay: bool) returns (br: BloodRecord)
+  //requires validDate(dd, mm, yy)
+  requires 0 < dd1 <= 31
+  requires 0 < mm1 <= 12
+  requires 0 < yy1 <= 2019
+  requires 0 < dd2 <= 31
+  requires 0 < mm2 <= 12
+  requires 0 < yy2 <= 2019
   {
     var d1: D.Date, d2: D.Date;
-    d1 := D.create(day1,month1,yr1);
-    d2 := D.create(day2,month2,yr2);
+    assert (0 < dd1 <= 31);
+    assert (0 < mm1 <= 12);
+    assert (0 < yy1 <= 2019);
+
+    assert (0 < dd2 <= 31);
+    assert (0 < mm2 <= 12);
+    assert (0 < yy2 <= 2019);
+
+    d1 := D.create(dd1,mm1,yy1);
+    d2 := D.create(dd2,mm2,yy2);
     return BloodRecord(bt, l, d1, d2, isOkay);
   }
 
+
   method hasExpired(b1: BloodRecord) returns (b: bool)
+  ensures b <==> D.current.
+  ensures b <==> (D.current.year < b1.expiryDate.year) 
+                       || (D.current.year == b1.expiryDate.year && D.current.month < b1.expiryDate.month) 
+                       || (D.current.year == b1.expiryDate.year && D.current.month == b1.expiryDate.month && D.current.day < b1.expiryDate.day)  
   {
-    var current := D.current();
-    return D.LessThan(current, b1.expiryDate);
+    b := D.lessThan(D.current, b1.expiryDate);
+    b := !b;
+    // This is stupid 
+    // Pls fix if you know how to do it :c
+  }
+
+  method compare(b1: BloodRecord, b2: BloodRecord) returns (cmp: int)
+  ensures (cmp == -1) ==> (b1.expiryDate.year < b2.expiryDate.year) 
+                       || (b1.expiryDate.year == b2.expiryDate.year && b1.expiryDate.month < b2.expiryDate.month) 
+                       || (b1.expiryDate.year == b2.expiryDate.year && b1.expiryDate.month == b2.expiryDate.month && b1.expiryDate.day < b2.expiryDate.day)  
+  ensures (cmp == 0) ==> (b1.expiryDate.year == b2.expiryDate.year && b1.expiryDate.month == b2.expiryDate.month && b1.expiryDate.day == b2.expiryDate.day)
+
+  ensures (cmp == 1) ==> (b2.expiryDate.year < b1.expiryDate.year) 
+                       || (b2.expiryDate.year == b1.expiryDate.year && b2.expiryDate.month < b1.expiryDate.month) 
+                       || (b2.expiryDate.year == b1.expiryDate.year && b2.expiryDate.month == b1.expiryDate.month && b2.expiryDate.day < b1.expiryDate.day)
+  {
+    var a := D.lessThan(b1.expiryDate, b2.expiryDate);
+    var b := D.lessThan(b2.expiryDate, b1.expiryDate);
+    assert( a ==> !b && b ==> !a);
+    if (a) { return -1; } 
+    else if (b) { return 1; }
+    else { return 0; }
+  }
+  
+  method Test() 
+  {
+    var typeA := createBt(0);
+    var typeB := createBt(1);
+    var typeAB := createBt(2);
+    var typeO := createBt(3);
+    
+    var br1 := createBr(typeA, "Backyard", 4, 2, 2003, 12, 4, 2007, true);
+    var br2 := createBr(typeA, "Backyard", 1, 2, 2013, 11, 5, 2015, true);
+    var br3 := createBr(typeA, "Backyard", 17, 5, 2014, 1, 7, 2016, true);
+
+    var test1 := hasExpired(br1);
+    var test2 := compare(br1, br1);
+    var test3 := compare(br1, br2);
+    var test4 := compare(br2, br1);
+
+    assert(test1);
+    
+    assert(test2 == 0); 
+    assert(test3 == -1);
+    assert(test4 == 1);
+    
   }
 }
+
